Loom/WP/SimpLemmas.lean
@@ -7,65 +7,51 @@ namespace Loom.WP
 universe u v
 variable {m : Type u → Type v}
 
-/-!
-# Simp lemmas for weakest preconditions
-
-This file provides simp lemmas for simplifying weakest precondition expressions.
-Unlike Std/Do, we use direct function application `wp x post epost` without notation.
-
-Some lemmas prove only one direction (`⊑`) instead of equality because our wp_bind axiom
-only provides one direction.
-TODO SG: These are useless. I think the whole file should actually be reformulated in terms of
-`simp` lemmas on monadic expressions, in a similar way to `ExceptT.run_bind`.
-The `simp` theory should apply to `wp` via `apply_wp` simp lemmas.
-I think that would be a worthwhile and reusable refactoring once we upstream.
--/
-
 /-! ## Basic WPMonad simp lemmas -/
 
 @[simp]
-theorem pure_wp [Monad m] [CompleteLattice l] [WPMonad m l e] (a : α) :
-  post a ⊑ wp (pure (f:=m) a) post epost := by
-  exact WPMonad.wp_pure a post epost
+theorem pure_wp [Monad m] [CompleteLattice l] [WPMonad m l es]
+    (a : α) (post : α → l) (epost : EPost es) :
+  post a ⊑ wp (pure (f := m) a) post epost :=
+  WPMonad.wp_pure a post epost
 
 @[simp]
-theorem bind_wp [Monad m] [CompleteLattice l] [WPMonad m l e] (x : m α) (f : α → m β) :
-  wp x (fun a => wp (f a) post epost) epost ⊑ wp (x >>= f) post epost := by
-  exact WPMonad.wp_bind x f post epost
-
--- Note: wp_map and wp_seq already exist in Basic.lean but without @[simp]
--- We re-export them here with the simp attribute
+theorem bind_wp [Monad m] [CompleteLattice l] [WPMonad m l es]
+    (x : m α) (f : α → m β) (post : β → l) (epost : EPost es) :
+  wp x (fun a => wp (f a) post epost) epost ⊑ wp (x >>= f) post epost :=
+  WPMonad.wp_bind x f post epost
 
 @[simp]
-theorem map_wp [Monad m] [LawfulMonad m] [CompleteLattice l] [WPMonad m l e] (f : α → β) (x : m α) :
+theorem map_wp [Monad m] [LawfulMonad m] [CompleteLattice l] [WPMonad m l es]
+    (f : α → β) (x : m α) (post : β → l) (epost : EPost es) :
   wp x (fun a => post (f a)) epost ⊑ wp (f <$> x) post epost :=
-  WPMonad.wp_map f x _ _
+  WPMonad.wp_map f x post epost
 
 @[simp]
-theorem seq_wp [Monad m] [LawfulMonad m] [CompleteLattice l] [WPMonad m l e] (f : m (α → β)) (x : m α) :
-  ∀ post epost, wp f (fun g => wp x (fun a => post (g a)) epost) epost ⊑ wp (f <*> x) post epost :=
-  WPMonad.wp_seq f x
+theorem seq_wp [Monad m] [LawfulMonad m] [CompleteLattice l] [WPMonad m l es]
+    (f : m (α → β)) (x : m α) (post : β → l) (epost : EPost es) :
+  wp f (fun g => wp x (fun a => post (g a)) epost) epost ⊑ wp (f <*> x) post epost :=
+  WPMonad.wp_seq f x post epost
 
-/-! ## MonadReaderOf simp lemmas -/
+/-! ## Reader / State simp lemmas -/
 
 @[simp]
-theorem read_ReaderT_wp [Monad m] [LawfulMonad m] [CompleteLattice l] [WPMonad m l e]
-    (post : ρ → ρ → l) (epost : e) :
+theorem read_ReaderT_wp [Monad m] [LawfulMonad m] [CompleteLattice l] [WPMonad m l es]
+    (post : ρ → ρ → l) (epost : EPost es) :
   (fun r => post r r) ⊑ wp (MonadReaderOf.read : ReaderT ρ m ρ) post epost := by
   intro r
   simpa [MonadReaderOf.read] using
     (WPMonad.wp_pure (m := m) (x := r) (post := fun a => post a r) (epost := epost))
 
 @[simp]
-theorem adapt_ReaderT_wp [Monad m] [LawfulMonad m] [CompleteLattice l] [WPMonad m l e] (f : ρ → ρ') (x : ReaderT ρ' m α) :
+theorem adapt_ReaderT_wp [Monad m] [LawfulMonad m] [CompleteLattice l] [WPMonad m l es]
+    (f : ρ → ρ') (x : ReaderT ρ' m α) (post : α → ρ → l) (epost : EPost es) :
   wp (ReaderT.adapt f x : ReaderT ρ m α) post epost =
     fun r => wp x (fun a _ => post a r) epost (f r) := rfl
 
-/-! ## MonadStateOf simp lemmas -/
-
 @[simp]
-theorem get_StateT_wp [Monad m] [LawfulMonad m] [CompleteLattice l] [WPMonad m l e]
-    (post : σ → σ → l) (epost : e) :
+theorem get_StateT_wp [Monad m] [LawfulMonad m] [CompleteLattice l] [WPMonad m l es]
+    (post : σ → σ → l) (epost : EPost es) :
   (fun s => post s s) ⊑ wp (MonadStateOf.get : StateT σ m σ) post epost := by
   intro s
   simpa [MonadStateOf.get] using
@@ -73,8 +59,8 @@ theorem get_StateT_wp [Monad m] [LawfulMonad m] [CompleteLattice l] [WPMonad m l
       (post := fun x => post x.fst x.snd) (epost := epost))
 
 @[simp]
-theorem set_StateT_wp [Monad m] [LawfulMonad m] [CompleteLattice l] [WPMonad m l e] (x : σ)
-    (post : PUnit → σ → l) (epost : e) :
+theorem set_StateT_wp [Monad m] [LawfulMonad m] [CompleteLattice l] [WPMonad m l es]
+    (x : σ) (post : PUnit → σ → l) (epost : EPost es) :
   (fun _ => post ⟨⟩ x) ⊑ wp (MonadStateOf.set x : StateT σ m PUnit) post epost := by
   intro s
   simpa [MonadStateOf.set] using
@@ -82,8 +68,8 @@ theorem set_StateT_wp [Monad m] [LawfulMonad m] [CompleteLattice l] [WPMonad m l
       (post := fun x => post x.fst x.snd) (epost := epost))
 
 @[simp]
-theorem modifyGet_StateT_wp [Monad m] [LawfulMonad m] [CompleteLattice l] [WPMonad m l e] (f : σ → α × σ)
-    (post : α → σ → l) (epost : e) :
+theorem modifyGet_StateT_wp [Monad m] [LawfulMonad m] [CompleteLattice l] [WPMonad m l es]
+    (f : σ → α × σ) (post : α → σ → l) (epost : EPost es) :
   (fun s => post (f s).1 (f s).2) ⊑ wp (MonadStateOf.modifyGet f : StateT σ m α) post epost := by
   intro s
   simpa [MonadStateOf.modifyGet] using
@@ -91,103 +77,71 @@ theorem modifyGet_StateT_wp [Monad m] [LawfulMonad m] [CompleteLattice l] [WPMon
       (post := fun x => post x.fst x.snd) (epost := epost))
 
 @[simp]
-theorem get_EStateM_wp :
+theorem get_EStateM_wp (post : σ → σ → Prop) (epost : EPost [ε → σ → Prop]) :
   wp (MonadStateOf.get : EStateM ε σ σ) post epost = fun s => post s s := by
   funext s
-  simp only [wp, WPMonad.wpImpl, MonadStateOf.get, EStateM.get] -- Would be nicer with a simp lemma for EStateM.wp
+  simp only [wp, WPMonad.wpImpl, MonadStateOf.get, EStateM.get]
 
 @[simp]
-theorem set_EStateM_wp (x : σ) :
+theorem set_EStateM_wp (x : σ) (post : PUnit → σ → Prop) (epost : EPost [ε → σ → Prop]) :
   wp (MonadStateOf.set x : EStateM ε σ PUnit) post epost = fun _ => post ⟨⟩ x := by
   funext s
   simp only [wp, WPMonad.wpImpl, MonadStateOf.set, EStateM.set]
 
 @[simp]
-theorem modifyGet_EStateM_wp (f : σ → α × σ) :
+theorem modifyGet_EStateM_wp (f : σ → α × σ) (post : α → σ → Prop) (epost : EPost [ε → σ → Prop]) :
   wp (MonadStateOf.modifyGet f : EStateM ε σ α) post epost = fun s => post (f s).1 (f s).2 := by
   funext s
   simp only [wp, WPMonad.wpImpl, MonadStateOf.modifyGet, EStateM.modifyGet]
 
-@[simp]
-theorem modify_StateT_wp [Monad m] [LawfulMonad m] [CompleteLattice l] [WPMonad m l e] (f : σ → σ) :
-  wp (modify f : StateT σ m PUnit) post epost =
-    wp (MonadStateOf.modifyGet fun s => (⟨⟩, f s) : StateT σ m PUnit) post epost := by
-  rfl
+/-! ## Except / throw / tryCatch simp lemmas -/
 
 @[simp]
-theorem getModify_StateT_wp [Monad m] [LawfulMonad m] [CompleteLattice l] [WPMonad m l e] (f : σ → σ) :
-  wp (getModify f : StateT σ m σ) post epost =
-    wp (MonadStateOf.modifyGet fun s => (s, f s) : StateT σ m σ) post epost := by
-  rfl
+theorem throwThe_wp [MonadExceptOf ε m] [Monad m] [CompleteLattice l] [WPMonad m l es]
+    (err : ε) (post : α → l) (epost : EPost es) :
+  wp (throwThe ε err : m α) post epost = wp (MonadExceptOf.throw err : m α) post epost := rfl
 
 @[simp]
-theorem modify_EStateM_wp (f : σ → σ) :
-  wp (modify f : EStateM ε σ PUnit) post epost =
-    wp (MonadStateOf.modifyGet fun s => (⟨⟩, f s) : EStateM ε σ PUnit) post epost := by
-  rfl
-
-@[simp]
-theorem getModify_EStateM_wp (f : σ → σ) :
-  wp (getModify f : EStateM ε σ σ) post epost =
-    wp (MonadStateOf.modifyGet fun s => (s, f s) : EStateM ε σ σ) post epost := by
-  rfl
-
-/-! ## MonadExceptOf simp lemmas -/
-
-@[simp]
-theorem throwThe_wp [MonadExceptOf ε m] [Monad m] [CompleteLattice l] [WPMonad m l e] (err : ε) :
-  wp (throwThe ε err : m α) post epost =
-    wp (MonadExceptOf.throw err : m α) post epost := by
-  rfl
-
-@[simp]
-theorem throw_Except_wp (e : ε) : wp (MonadExceptOf.throw e : Except ε α) post epost = epost.2 e := by
-  -- TODO: better: Define `WPMonad Except` in terms of `pushExcept (pure x)`, define simp lemma and use it here
+theorem throw_Except_wp (e : ε) (post : α → Prop) (epost : EPost [ε → Prop]) :
+  wp (MonadExceptOf.throw e : Except ε α) post epost = epost.head e := by
   simp [wp, WPMonad.wpImpl]
 
 @[simp]
-theorem throw_ExceptT_wp [Monad m] [LawfulMonad m] [CompleteLattice l] [WPMonad m l e] (err : ε) :
-  epost.2 err ⊑ wp (MonadExceptOf.throw err : ExceptT ε m α) post epost := by
+theorem throw_ExceptT_wp [Monad m] [LawfulMonad m] [CompleteLattice l] [WPMonad m l es]
+    (err : ε) (post : α → l) (epost : EPost ((ε → l) :: es)) :
+  epost.head err ⊑ wp (MonadExceptOf.throw err : ExceptT ε m α) post epost := by
   simpa [MonadExceptOf.throw, pushExcept.post] using
     (WPMonad.wp_pure (m := m) (x := Except.error err)
-      (post := pushExcept.post post epost) (epost := epost.1))
+      (post := pushExcept.post post epost) (epost := epost.tail))
 
 @[simp]
-theorem throw_EStateM_wp (e : ε) :
-  wp (MonadExceptOf.throw e : EStateM ε σ α) post epost = epost e := by
+theorem throw_EStateM_wp (e : ε) (post : α → σ → Prop) (epost : EPost [ε → σ → Prop]) :
+  wp (MonadExceptOf.throw e : EStateM ε σ α) post epost = fun s => epost.head e s := by
   funext s
   simp only [wp, WPMonad.wpImpl, MonadExceptOf.throw, EStateM.throw]
 
 @[simp]
-theorem throw_Option_wp (e : PUnit) : wp (MonadExceptOf.throw e : Option α) post epost = epost := by
+theorem throw_Option_wp (e : PUnit) (post : α → Prop) (epost : EPost [Prop]) :
+  wp (MonadExceptOf.throw e : Option α) post epost = epost.head := by
+  cases e
   simp only [wp, MonadExceptOf.throw]
   rfl
 
-/-
 @[simp]
-theorem throw_OptionT_wp [Monad m] [LawfulMonad m] [CompleteLattice l] [WPMonad m l e] (err : PUnit) :
-  wp (MonadExceptOf.throw err : OptionT m α) post epost = epost.2 := by
-  simp only [wp, MonadExceptOf.throw, OptionT.mk, OptionT.fail, OptionT.run, WPMonad.wp_pure]
--/
+theorem tryCatch_MonadExcept_wp [MonadExceptOf ε m] [Monad m] [CompleteLattice l] [WPMonad m l es]
+    (x : m α) (h : ε → m α) (post : α → l) (epost : EPost es) :
+  wp (tryCatch x h : m α) post epost = wp (MonadExceptOf.tryCatch x h : m α) post epost := rfl
 
 @[simp]
-theorem tryCatch_MonadExcept_wp [MonadExceptOf ε m] [Monad m] [CompleteLattice l] [WPMonad m l e] (x : m α) (h : ε → m α) :
-  wp (tryCatch x h : m α) post epost =
-    wp (MonadExceptOf.tryCatch x h : m α) post epost := by
-  rfl
+theorem tryCatchThe_wp [MonadExceptOf ε m] [Monad m] [CompleteLattice l] [WPMonad m l es]
+    (x : m α) (h : ε → m α) (post : α → l) (epost : EPost es) :
+  wp (tryCatchThe ε x h : m α) post epost = wp (MonadExceptOf.tryCatch x h : m α) post epost := rfl
 
 @[simp]
-theorem tryCatchThe_wp [MonadExceptOf ε m] [Monad m] [CompleteLattice l] [WPMonad m l e] (x : m α) (h : ε → m α) :
-  wp (tryCatchThe ε x h : m α) post epost =
-    wp (MonadExceptOf.tryCatch x h : m α) post epost := by
-  rfl
-
-@[simp]
-theorem tryCatch_Except_wp (x : Except ε α) (h : ε → Except ε α) :
+theorem tryCatch_Except_wp (x : Except ε α) (h : ε → Except ε α) (post : α → Prop) (epost : EPost [ε → Prop]) :
   wp (MonadExceptOf.tryCatch x h : Except ε α) post epost =
-    wp x post (.unit, fun e => wp (h e) post epost) := by
-  simp only [wp, WPMonad.wpImpl, MonadExceptOf.tryCatch, Except.tryCatch]
-  cases x <;> simp
+    wp x post epost⟨fun e => wp (h e) post epost⟩ := by
+  cases x <;> rfl
 
 -- TODO: Upstream
 @[simp] theorem _root_.ExceptT.run_tryCatch [Monad m] [LawfulMonad m] (x : ExceptT ε m α) (h : ε → ExceptT ε m α) :
@@ -201,491 +155,89 @@ theorem tryCatch_Except_wp (x : Except ε α) (h : ε → Except ε α) :
   rfl
 
 @[simp]
-theorem tryCatch_ExceptT_wp [Monad m] [LawfulMonad m] [CompleteLattice l] [WPMonad m l e] (x : ExceptT ε m α) (h : ε → ExceptT ε m α) :
-  wp x post (epost.1, fun e => wp (h e) post epost) ⊑
-  wp (MonadExceptOf.tryCatch x h : ExceptT ε m α) post epost
-     := by
+theorem tryCatch_ExceptT_wp [Monad m] [LawfulMonad m] [CompleteLattice l] [WPMonad m l es]
+    (x : ExceptT ε m α) (h : ε → ExceptT ε m α) (post : α → l) (epost : EPost ((ε → l) :: es)) :
+  wp x post (EPost.cons (fun e => wp (h e) post epost) epost.tail) ⊑
+    wp (MonadExceptOf.tryCatch x h : ExceptT ε m α) post epost := by
   change _ ⊑ wp (tryCatch x h : ExceptT ε m α) _ _
   simp only [ExceptT.apply_wp, ExceptT.run_tryCatch]
-  apply PartialOrder.rel_trans; rotate_left; apply WPMonad.wp_bind
-  apply WPMonad.wp_cons; intro r; cases r with
-  | ok a => simpa [pushExcept.post] using
-      (WPMonad.wp_pure (m := m) (x := Except.ok a)
-        (post := pushExcept.post post epost) (epost := epost.1))
-  | error _ => exact PartialOrder.rel_refl
-
-/-
-@[simp]
-theorem tryCatch_Option_wp (x : Option α) (h : PUnit → Option α) :
-  wp (MonadExceptOf.tryCatch x h : Option α) post epost =
-    wp x post (wp (h ⟨⟩) post epost) := by
-  simp only [wp, MonadExceptOf.tryCatch, Option.tryCatch]
-  cases x <;> simp
--/
+  apply PartialOrder.rel_trans; rotate_left
+  · apply WPMonad.wp_bind
+  · apply WPMonad.wp_cons
+    intro r; cases r with
+    | ok a => simpa [pushExcept.post] using
+        (WPMonad.wp_pure (m := m) (x := Except.ok a)
+          (post := pushExcept.post post epost) (epost := epost.tail))
+    | error _ => exact PartialOrder.rel_refl
 
 @[simp]
-theorem tryCatch_EStateM_wp (x : EStateM ε σ α) (h : ε → EStateM ε σ α) :
+theorem tryCatch_EStateM_wp (x : EStateM ε σ α) (h : ε → EStateM ε σ α)
+    (post : α → σ → Prop) (epost : EPost [ε → σ → Prop]) :
   wp (MonadExceptOf.tryCatch x h : EStateM ε σ α) post epost =
-    fun s => wp x post (fun e s' => wp (h e) post epost s') s := by
+    fun s => wp x post epost⟨fun e s' => wp (h e) post epost s'⟩ s := by
   funext s
   simp only [wp, WPMonad.wpImpl, MonadExceptOf.tryCatch, EStateM.tryCatch]
   cases (x s) <;> simp
   rfl
 
-/-
-@[simp]
-theorem tryCatch_OptionT_wp [Monad m] [LawfulMonad m] [CompleteLattice l] [WPMonad m l e] (x : OptionT m α) (h : PUnit → OptionT m α) :
-  wp x post (epost.1, wp (h ⟨⟩) post epost) ⊑
-    wp (MonadExceptOf.tryCatch x h : OptionT m α) post epost := by
-  simp only [wp, MonadExceptOf.tryCatch, OptionT.tryCatch, OptionT.mk, OptionT.run]
-  apply PartialOrder.rel_trans; rotate_left; apply WPMonad.wp_bind
-  apply WPMonad.wp_cons (m := m); intro o; cases o with
-  | some a => simp [WPMonad.wp_pure (m := m), PartialOrder.rel_refl]
-  | none => exact PartialOrder.rel_refl
--/
-
 /-! ## Additional state operation lemmas -/
 
 @[simp]
-theorem getThe_StateT_wp [Monad m] [LawfulMonad m] [CompleteLattice l] [WPMonad m l e] :
-  wp (getThe σ : StateT σ m σ) post epost =
-    wp (MonadStateOf.get : StateT σ m σ) post epost := by
-  rfl
+theorem getThe_StateT_wp [Monad m] [LawfulMonad m] [CompleteLattice l] [WPMonad m l es]
+    (post : σ → σ → l) (epost : EPost es) :
+  wp (getThe σ : StateT σ m σ) post epost = wp (MonadStateOf.get : StateT σ m σ) post epost := rfl
 
 @[simp]
-theorem modifyThe_StateT_wp [Monad m] [LawfulMonad m] [CompleteLattice l] [WPMonad m l e] (f : σ → σ) :
+theorem modifyThe_StateT_wp [Monad m] [LawfulMonad m] [CompleteLattice l] [WPMonad m l es]
+    (f : σ → σ) (post : PUnit → σ → l) (epost : EPost es) :
   wp (modifyThe σ f : StateT σ m PUnit) post epost =
-    wp (MonadStateOf.modifyGet fun s => (⟨⟩, f s) : StateT σ m PUnit) post epost := by
-  rfl
+    wp (MonadStateOf.modifyGet fun s => (⟨⟩, f s) : StateT σ m PUnit) post epost := rfl
 
 @[simp]
-theorem modifyGetThe_StateT_wp [Monad m] [LawfulMonad m] [CompleteLattice l] [WPMonad m l e] (f : σ → α × σ) :
+theorem modifyGetThe_StateT_wp [Monad m] [LawfulMonad m] [CompleteLattice l] [WPMonad m l es]
+    (f : σ → α × σ) (post : α → σ → l) (epost : EPost es) :
   wp (modifyGetThe σ f : StateT σ m α) post epost =
-    wp (MonadStateOf.modifyGet f : StateT σ m α) post epost := by
-  rfl
-
-@[simp]
-theorem get_MonadState_wp [Monad m] [LawfulMonad m] [CompleteLattice l] [WPMonad m l e] [MonadStateOf σ m] :
-  wp (MonadState.get : m σ) post epost =
-    wp (MonadStateOf.get : m σ) post epost := by
-  rfl
-
-@[simp]
-theorem set_MonadState_wp [Monad m] [LawfulMonad m] [CompleteLattice l] [WPMonad m l e] [MonadStateOf σ m] (x : σ) :
-  wp (MonadState.set x : m PUnit) post epost =
-    wp (MonadStateOf.set x : m PUnit) post epost := by
-  rfl
-
-@[simp]
-theorem modifyGet_MonadState_wp [Monad m] [LawfulMonad m] [CompleteLattice l] [WPMonad m l e] [MonadStateOf σ m] (f : σ → α × σ) :
-  wp (MonadState.modifyGet f : m α) post epost =
-    wp (MonadStateOf.modifyGet f : m α) post epost := by
-  rfl
-
-@[simp]
-theorem read_MonadReader_wp [Monad m] [LawfulMonad m] [CompleteLattice l] [WPMonad m l e] [MonadReaderOf ρ m] :
-  wp (MonadReader.read : m ρ) post epost =
-    wp (MonadReaderOf.read : m ρ) post epost := by
-  rfl
-
-@[simp]
-theorem readThe_ReaderT_wp [Monad m] [LawfulMonad m] [CompleteLattice l] [WPMonad m l e] :
-  wp (readThe ρ : ReaderT ρ m ρ) post epost =
-    wp (MonadReaderOf.read : ReaderT ρ m ρ) post epost := by
-  rfl
+    wp (MonadStateOf.modifyGet f : StateT σ m α) post epost := rfl
 
 /-! ## MonadLift simp lemmas -/
 
 @[simp]
-theorem monadLift_StateT_wp [Monad m] [LawfulMonad m] [CompleteLattice l] [WPMonad m l e] (x : m α) (post : α → σ → l) :
+theorem monadLift_StateT_wp [Monad m] [LawfulMonad m] [CompleteLattice l] [WPMonad m l es]
+    (x : m α) (post : α → σ → l) (epost : EPost es) :
   (fun s => wp x (fun a => post a s) epost) ⊑
     wp (MonadLift.monadLift x : StateT σ m α) post epost := by
   intro s
   simp only [wp, MonadLift.monadLift]
-  apply PartialOrder.rel_trans; rotate_left; apply WPMonad.wp_bind
-  apply WPMonad.wp_cons (m := m); intro a
-  simpa using
-    (WPMonad.wp_pure (m := m) (x := (a, s))
-      (post := fun x => post x.fst x.snd) (epost := epost))
+  apply PartialOrder.rel_trans; rotate_left
+  · apply WPMonad.wp_bind
+  · apply WPMonad.wp_cons (m := m)
+    intro a
+    simpa using
+      (WPMonad.wp_pure (m := m) (x := (a, s))
+        (post := fun x => post x.fst x.snd) (epost := epost))
 
 @[simp]
-theorem monadLift_ReaderT_wp [Monad m] [LawfulMonad m] [CompleteLattice l] [WPMonad m l e] (x : m α) :
-  wp (MonadLift.monadLift x : ReaderT ρ m α) post epost =
-    fun r => wp x (fun a => post a r) epost := by
-  rfl
+theorem monadLift_ReaderT_wp [Monad m] [LawfulMonad m] [CompleteLattice l] [WPMonad m l es]
+    (x : m α) (post : α → ρ → l) (epost : EPost es) :
+  wp (MonadLift.monadLift x : ReaderT ρ m α) post epost = fun r => wp x (fun a => post a r) epost := rfl
 
 @[simp]
-theorem monadLift_ExceptT_wp [Monad m] [LawfulMonad m] [CompleteLattice l] [WPMonad m l e] (x : m α) (post : α → l) (epost : e × (ε → l)) :
-  wp x post epost.1 ⊑
-    wp (MonadLift.monadLift x : ExceptT ε m α) post epost := by
+theorem monadLift_ExceptT_wp [Monad m] [LawfulMonad m] [CompleteLattice l] [WPMonad m l es]
+    (x : m α) (post : α → l) (epost : EPost ((ε → l) :: es)) :
+  wp x post epost.tail ⊑ wp (MonadLift.monadLift x : ExceptT ε m α) post epost := by
   simp only [wp, MonadLift.monadLift, ExceptT.lift, ExceptT.mk]
   apply PartialOrder.rel_trans; rotate_left
   · exact WPMonad.wp_map (m := m) Except.ok x _ _
   · exact PartialOrder.rel_refl
 
 @[simp]
-theorem lift_StateT_wp [Monad m] [LawfulMonad m] [CompleteLattice l] [WPMonad m l e] (x : m α) :
-  wp (StateT.lift x : StateT σ m α) post epost =
-    wp (MonadLift.monadLift x : StateT σ m α) post epost := by
-  rfl
+theorem lift_StateT_wp [Monad m] [LawfulMonad m] [CompleteLattice l] [WPMonad m l es]
+    (x : m α) (post : α → σ → l) (epost : EPost es) :
+  wp (StateT.lift x : StateT σ m α) post epost = wp (MonadLift.monadLift x : StateT σ m α) post epost := rfl
 
 @[simp]
-theorem lift_ExceptT_wp [Monad m] [LawfulMonad m] [CompleteLattice l] [WPMonad m l e] (x : m α) :
-  wp (ExceptT.lift x : ExceptT ε m α) post epost =
-    wp (MonadLift.monadLift x : ExceptT ε m α) post epost := by
-  rfl
-
-/-
-@[simp]
-theorem monadLift_OptionT_wp [Monad m] [LawfulMonad m] [CompleteLattice l] [WPMonad m l e] (x : m α) :
-  wp x post epost.1 ⊑
-    wp (MonadLift.monadLift x : OptionT m α) post epost := by
-  simp only [wp, MonadLift.monadLift, OptionT.mk, OptionT.lift, OptionT.run]
-  apply PartialOrder.rel_trans; rotate_left; apply WPMonad.wp_bind
-  apply WPMonad.wp_cons (m := m); intro a
-  simp [WPMonad.wp_pure (m := m), PartialOrder.rel_refl]
--/
-
-@[simp]
-theorem lift_OptionT_wp [Monad m] [LawfulMonad m] [CompleteLattice l] [WPMonad m l e] [WPMonad (OptionT m) l (e × l)] (x : m α) :
-  wp (OptionT.lift x : OptionT m α) post epost =
-    wp (MonadLift.monadLift x : OptionT m α) post epost := rfl
-
-/-! ## MonadFunctor simp lemmas -/
-
-@[simp]
-theorem monadMap_StateT_wp [Monad m] [LawfulMonad m] [CompleteLattice l] [WPMonad m l e]
-  (f : ∀{β}, m β → m β) {α} (x : StateT σ m α) (post : α → σ → l) (epost : e) :
-  wp (MonadFunctor.monadMap (m:=m) f x : StateT σ m α) post epost =
-    fun s => wp (f (x.run s)) (fun (a, s') => post a s') epost := by
-  funext s
-  simp [MonadFunctor.monadMap, StateT.run]
-
-@[simp]
-theorem monadMap_ReaderT_wp [Monad m] [LawfulMonad m] [CompleteLattice l] [WPMonad m l e]
-  (f : ∀{β}, m β → m β) {α} (x : ReaderT ρ m α) (post : α → ρ → l) (epost : e) :
-  wp (MonadFunctor.monadMap (m:=m) f x : ReaderT ρ m α) post epost =
-    fun r => wp (f (x.run r)) (fun a => post a r) epost := by
-  funext r
-  simp [MonadFunctor.monadMap, ReaderT.run]
-
-@[simp]
-theorem monadMap_ExceptT_wp [Monad m] [LawfulMonad m] [CompleteLattice l] [WPMonad m l e]
-  (f : ∀{β}, m β → m β) {α} (x : ExceptT ε m α) (post : α → l) (epost : e × (ε → l)) :
-  wp (MonadFunctor.monadMap (m:=m) f x : ExceptT ε m α) post epost =
-    wp (f x.run) (pushExcept.post post epost) epost.1 := by
-  simp [MonadFunctor.monadMap, ExceptT.run]
-
-/-
-@[simp]
-theorem monadMap_OptionT_wp [Monad m] [LawfulMonad m] [CompleteLattice l] [WPMonad m l e]
-  (f : ∀{β}, m β → m β) {α} (x : OptionT m α) (post : α → l) (epost : e × l) :
-  wp (MonadFunctor.monadMap (m:=m) f x : OptionT m α) post epost =
-    wp (f x.run) (fun o => match o with | some a => post a | none => epost.2) epost.1 := by
-  simp only [wp, MonadFunctor.monadMap, OptionT.run]; rfl
--/
-
-@[simp]
-theorem withReader_ReaderT_wp [Monad m] [LawfulMonad m] [CompleteLattice l] [WPMonad m l e] (f : ρ → ρ) (x : ReaderT ρ m α) :
-  wp (MonadWithReaderOf.withReader f x : ReaderT ρ m α) post epost =
-    fun r => wp x (fun a _ => post a r) epost (f r) := rfl
-
-@[simp]
-theorem withReader_MonadWithReader_wp [Monad m] [LawfulMonad m] [CompleteLattice l] [WPMonad m l e] [MonadWithReaderOf ρ m] (f : ρ → ρ) (x : m α) :
-  wp (MonadWithReader.withReader f x : m α) post epost =
-    wp (MonadWithReaderOf.withReader f x : m α) post epost := rfl
-
-@[simp]
-theorem withTheReader_ReaderT_wp [Monad m] [LawfulMonad m] [CompleteLattice l] [WPMonad m l e] (f : ρ → ρ) (x : ReaderT ρ m α) :
-  wp (withTheReader ρ f x : ReaderT ρ m α) post epost =
-    wp (MonadWithReaderOf.withReader f x : ReaderT ρ m α) post epost := rfl
-
-/-! ## Transformer adapt lemmas -/
-
-@[simp]
-theorem adapt_ExceptT_wp [Monad m] [LawfulMonad m] [CompleteLattice l] [WPMonad m l e] (f : ε → ε') (x : ExceptT ε m α) :
-  wp x post (epost.1, fun e => epost.2 (f e)) ⊑
-    wp (ExceptT.adapt f x : ExceptT ε' m α) post epost := by
-  simp only [wp, ExceptT.adapt, ExceptT.mk]
-  apply PartialOrder.rel_trans; rotate_left
-  · exact WPMonad.wp_map (m := m) (Except.mapError f) x _ _
-  · apply WPMonad.wp_cons (m := m); intro r; cases r <;> exact PartialOrder.rel_refl
-
-@[simp]
-theorem adaptExcept_EStateM_wp (f : ε → ε') (x : EStateM ε σ α) :
-  wp (EStateM.adaptExcept f x : EStateM ε' σ α) post epost =
-    wp x post (fun e => epost (f e)) := by
-  funext s
-  simp only [wp, WPMonad.wpImpl, EStateM.adaptExcept]
-  cases (x s) <;> simp
-
-/-! ## MonadControl simp lemmas -/
-
-@[simp]
-theorem liftWith_StateT_wp [Monad m] [LawfulMonad m] [CompleteLattice l] [WPMonad m l e]
-  (f : (∀{β}, StateT σ m β → m (β × σ)) → m α) :
-  wp (MonadControl.liftWith (m:=m) f : StateT σ m α) post epost s =
-    wp ((fun a => (a, s)) <$> f (fun x => x.run s)) (fun ⟨a, s⟩ => post a s) epost := by
-  simp [MonadControl.liftWith]
-
-@[simp]
-theorem liftWith_ReaderT_wp [Monad m] [LawfulMonad m] [CompleteLattice l] [WPMonad m l e]
-  (f : (∀{β}, ReaderT ρ m β → m β) → m α) :
-  wp (MonadControl.liftWith (m:=m) f : ReaderT ρ m α) post epost r =
-    wp (f (fun x => x.run r)) (fun a => post a r) epost := by
-  simp [MonadControl.liftWith, ReaderT.run]
-
--- TODO: Upstream
-@[simp] theorem _root_.ExceptT.run_liftM [Monad m] [LawfulMonad m] (x : m α) :
-  (liftM x : ExceptT ε m α).run = (Except.ok <$> x : m (Except ε α)) := rfl
-
-@[simp]
-theorem liftWith_ExceptT_wp [Monad m] [LawfulMonad m] [CompleteLattice l] [WPMonad m l e]
-  (f : (∀{β}, ExceptT ε m β → m (Except ε β)) → m α) :
-  wp (MonadControl.liftWith (m:=m) f : ExceptT ε m α) post epost =
-    wp (Except.ok <$> f (fun x => x.run)) (pushExcept.post post epost) epost.1 := by
-  change wp (liftWith (m:=m) f : ExceptT ε m α) post epost =
-    wp (Except.ok <$> f (fun x => x.run)) (pushExcept.post post epost) epost.1
-  simp
-
-/-
-@[simp]
-theorem liftWith_OptionT_wp [Monad m] [LawfulMonad m] [CompleteLattice l] [WPMonad m l e]
-  (f : (∀{β}, OptionT m β → m (Option β)) → m α) :
-  wp (f (fun x => x.run)) post epost.1 ⊑
-    wp (MonadControl.liftWith (m:=m) f : OptionT m α) post epost := by
-  simp [MonadControl.liftWith, liftM, monadLift]
--/
-
-@[simp]
-theorem restoreM_StateT_wp [Monad m] [LawfulMonad m] [CompleteLattice l] [WPMonad m l e] (x : m (α × σ)) :
-  (fun _ => wp x (fun (a, s) => post a s) epost) ⊑
-    wp (MonadControl.restoreM (m:=m) x : StateT σ m α) post epost := by
-  simp only [MonadControl.restoreM]
-  apply PartialOrder.rel_trans; rotate_left; apply WPMonad.wp_bind; simp only [liftM, monadLift]
-  apply PartialOrder.rel_trans; rotate_left; apply monadLift_StateT_wp
-  intro s; apply WPMonad.wp_cons; intro s'; simp only
-  apply PartialOrder.rel_trans; rotate_left; apply WPMonad.wp_bind
-  simp [set, StateT.set, pure, StateT.pure]
-  apply PartialOrder.rel_trans
-  · simpa using
-      (WPMonad.wp_pure (m := m) (x := (s'.fst, s'.snd))
-        (post := fun x => post x.fst x.snd) (epost := epost))
-  · simpa using
-      (WPMonad.wp_pure (m := m) (x := (PUnit.unit, s'.snd))
-        (post := fun x => wp (pure (s'.fst, x.snd)) (fun x => post x.fst x.snd) epost)
-        (epost := epost))
-
-@[simp]
-theorem restoreM_ReaderT_wp [Monad m] [LawfulMonad m] [CompleteLattice l] [WPMonad m l e] (x : m α) :
-  wp (MonadControl.restoreM (m:=m) x : ReaderT ρ m α) post epost =
-    fun r => wp x (fun a => post a r) epost := by
-  funext r
-  simp [MonadControl.restoreM, ReaderT.run]
-
-@[simp]
-theorem restoreM_ExceptT_wp [Monad m] [LawfulMonad m] [CompleteLattice l] [WPMonad m l e] (x : m (Except ε α)) :
-  wp (MonadControl.restoreM (m:=m) x : ExceptT ε m α) post epost =
-    wp x (pushExcept.post post epost) epost.1 := by
-  simp [MonadControl.restoreM, ExceptT.run]
-
-/-
-@[simp]
-theorem restoreM_OptionT_wp [Monad m] [LawfulMonad m] [CompleteLattice l] [WPMonad m l e] (x : m (Option α)) :
-  wp (MonadControl.restoreM (m:=m) x : OptionT m α) post epost =
-    wp x (pushOption.post post epost) epost.1 := by
-  simp only [wp, MonadControl.restoreM]; rfl
--/
-
-@[simp]
-theorem controlAt_wp [Bind n] [Monad n] [Monad m] [CompleteLattice l] [WPMonad n l e] [MonadControlT m n]
-  (f : (∀{β}, n β → m (stM m n β)) → m (stM m n α)) :
-  wp (controlAt m f : n α) post epost =
-    wp (liftWith f >>= restoreM : n α) post epost := by
-  rfl
-
-@[simp]
-theorem control_wp [Bind n] [Monad n] [Monad m] [CompleteLattice l] [WPMonad n l e] [MonadControlT m n]
-  (f : (∀{β}, n β → m (stM m n β)) → m (stM m n α)) :
-  wp (control f : n α) post epost =
-    wp (liftWith f >>= restoreM : n α) post epost := by
-  rfl
-
-@[simp]
-theorem monadLift_trans_wp [Monad o] [CompleteLattice l] [WPMonad o l e] [MonadLift n o] [MonadLiftT m n] (x : m α) :
-  wp (MonadLiftT.monadLift x : o α) post epost =
-    wp (MonadLift.monadLift (m:=n) (MonadLiftT.monadLift (m:=m) x) : o α) post epost := rfl
-
-@[simp]
-theorem monadLift_refl_wp [Monad m] [CompleteLattice l] [WPMonad m l e] (x : m α) :
-  wp (MonadLiftT.monadLift x : m α) post epost =
-    wp (x : m α) post epost := rfl
-
-@[simp]
-theorem monadMap_trans_wp [Monad o] [CompleteLattice l] [WPMonad o l e] [MonadFunctor n o] [MonadFunctorT m n] (x : o α) :
-  wp (MonadFunctorT.monadMap f x : o α) post epost =
-    wp (MonadFunctor.monadMap (m:=n) (MonadFunctorT.monadMap (m:=m) f) x : o α) post epost := by rfl
-
-@[simp]
-theorem monadMap_refl_wp [Monad m] [CompleteLattice l] [WPMonad m l e] (x : m α) :
-  wp (MonadFunctorT.monadMap f x : m α) post epost =
-    wp (f x : m α) post epost := by rfl
-
-
-@[simp]
-theorem get_MonadStateOf_lift_wp [MonadStateOf σ m] [MonadLift m n] [Monad m] [Monad n] [CompleteLattice l] [WPMonad n l e'] :
-  wp (MonadStateOf.get : n σ) post epost =
-    wp (MonadLift.monadLift (MonadStateOf.get : m σ) : n σ) post epost := by
-  rfl
-
-@[simp]
-theorem set_MonadStateOf_lift_wp [MonadStateOf σ m] [MonadLift m n] [Monad m] [Monad n] [CompleteLattice l] [WPMonad n l e'] (x : σ) :
-  wp (MonadStateOf.set x : n PUnit) post epost =
-    wp (MonadLift.monadLift (MonadStateOf.set (σ:=σ) x : m PUnit) : n PUnit) post epost := by
-  rfl
-
-@[simp]
-theorem modifyGet_MonadStateOf_lift_wp [MonadStateOf σ m] [MonadLift m n] [Monad m] [Monad n] [CompleteLattice l] [WPMonad n l e']
-  (f : σ → α × σ) :
-  wp (MonadStateOf.modifyGet f : n α) post epost =
-    wp (MonadLift.monadLift (MonadState.modifyGet f : m α) : n α) post epost := by
-  rfl
-
-@[simp]
-theorem read_MonadReaderOf_lift_wp [MonadReaderOf ρ m] [MonadLift m n] [Monad m] [Monad n] [CompleteLattice l] [WPMonad n l e'] :
-  wp (MonadReaderOf.read : n ρ) post epost =
-    wp (MonadLift.monadLift (MonadReader.read : m ρ) : n ρ) post epost := by
-  rfl
-
-@[simp]
-theorem throw_lift_ExceptT_wp [Monad m] [LawfulMonad m] [CompleteLattice l] [WPMonad m l e'] [MonadExceptOf ε m] (err : ε) :
-  wp (MonadExceptOf.throw (ε:=ε) err : ExceptT ε' m α) post epost =
-    wp (MonadExceptOf.throw (ε:=ε) err : m (Except ε' α)) (pushExcept.post post epost) epost.1 := by
-  rfl
-
-/-
-@[simp]
-theorem throw_lift_OptionT_wp [Monad m] [LawfulMonad m] [CompleteLattice l] [WPMonad m l e'] [MonadExceptOf ε m] (err : ε) :
-  wp (MonadExceptOf.throw (ε:=ε) err : OptionT m α) post epost =
-    wp (MonadExceptOf.throw (ε:=ε) err : m (Option α)) (fun o => match o with | some a => post a | none => epost.2) epost.1 := by
-  rfl
--/
-
-@[simp]
-theorem tryCatch_lift_ExceptT_wp [Monad m] [LawfulMonad m] [CompleteLattice l] [WPMonad m l e'] [MonadExceptOf ε m] (x : ExceptT ε' m α) (h : ε → ExceptT ε' m α) :
-  wp (MonadExceptOf.tryCatch (ε:=ε) x h : ExceptT ε' m α) post epost =
-    wp (MonadExceptOf.tryCatch (ε:=ε) x h : m (Except ε' α)) (pushExcept.post post epost) epost.1 := by
-  rfl
-
-/-
-@[simp]
-theorem tryCatch_lift_OptionT_wp [Monad m] [LawfulMonad m] [CompleteLattice l] [WPMonad m l e'] [MonadExceptOf ε m] (x : OptionT m α) (h : ε → OptionT m α) :
-  wp (MonadExceptOf.tryCatch (ε:=ε) x h : OptionT m α) post epost =
-    wp (MonadExceptOf.tryCatch (ε:=ε) x h : m (Option α)) (pushOption.post post epost) epost.1 := by
-  rfl
--/
-
-@[simp]
-theorem throw_ReaderT_lift_wp [Monad m] [LawfulMonad m] [CompleteLattice l] [WPMonad m l e'] [MonadExceptOf ε m] (err : ε) :
-  wp (MonadExceptOf.throw (ε:=ε) err : ReaderT ρ m α) post epost =
-    wp (MonadLift.monadLift (MonadExceptOf.throw (ε:=ε) err : m α) : ReaderT ρ m α) post epost := by
-  rfl
-
-@[simp]
-theorem throw_StateT_lift_wp [Monad m] [LawfulMonad m] [CompleteLattice l] [WPMonad m l e'] [MonadExceptOf ε m] (err : ε) :
-  wp (MonadExceptOf.throw (ε:=ε) err : StateT σ m α) post epost =
-    wp (MonadLift.monadLift (MonadExceptOf.throw (ε:=ε) err : m α) : StateT σ m α) post epost := by
-  rfl
-
-@[simp]
-theorem tryCatch_ReaderT_lift_wp [Monad m] [LawfulMonad m] [CompleteLattice l] [WPMonad m l e'] [MonadExceptOf ε m] (x : ReaderT ρ m α) (h : ε → ReaderT ρ m α) :
-  wp (MonadExceptOf.tryCatch (ε:=ε) x h : ReaderT ρ m α) post epost =
-    fun r => wp (MonadExceptOf.tryCatch (ε:=ε) (x.run r) (fun e => (h e).run r) : m α) (fun a => post a r) epost := by
-  rfl
-
-@[simp]
-theorem tryCatch_StateT_lift_wp [Monad m] [LawfulMonad m] [CompleteLattice l] [WPMonad m l e'] [MonadExceptOf ε m] (x : StateT σ m α) (h : ε → StateT σ m α) :
-  wp (MonadExceptOf.tryCatch (ε:=ε) x h : StateT σ m α) post epost =
-    fun s => wp (MonadExceptOf.tryCatch (ε:=ε) (x.run s) (fun e => (h e).run s) : m (α × σ)) (fun (a, s') => post a s') epost := by
-  rfl
-
-@[simp]
-theorem liftWith_trans_wp [Monad o] [CompleteLattice l] [WPMonad o l e] [MonadControl n o] [MonadControlT m n]
-  (f : (∀{β}, o β → m (stM m o β)) → m α) :
-  wp (MonadControlT.liftWith f : o α) post epost =
-    wp (MonadControl.liftWith (m:=n) fun x₂ => MonadControlT.liftWith fun x₁ => f (x₁ ∘ x₂) : o α) post epost := by
-  rfl
-
-@[simp]
-theorem liftWith_refl_wp [Pure m] [Monad m] [CompleteLattice l] [WPMonad m l e]
-  (f : (∀{β}, m β → m β) → m α) :
-  wp (MonadControlT.liftWith (m:=m) f : m α) post epost =
-    wp (f (fun x => x) : m α) post epost := by
-  rfl
-
-@[simp]
-theorem restoreM_trans_wp [Monad o] [CompleteLattice l] [WPMonad o l e] [MonadControl n o] [MonadControlT m n] (x : stM m o α) :
-  wp (MonadControlT.restoreM x : o α) post epost =
-    wp (MonadControl.restoreM (m:=n) (MonadControlT.restoreM (m:=m) x) : o α) post epost := by
-  rfl
-
-@[simp]
-theorem restoreM_refl_wp [Pure m] [Monad m] [CompleteLattice l] [WPMonad m l e] (x : stM m m α) :
-  wp (MonadControlT.restoreM x : m α) post epost =
-    wp (Pure.pure x : m α) post epost := by
-  rfl
-
-/-! ## OrElse simp lemmas -/
-
-@[simp]
-theorem orElse_Except_wp (x : Except ε α) (h : Unit → Except ε α) :
-  wp (OrElse.orElse x h : Except ε α) post epost =
-    wp x post (.unit, fun _ => wp (h ()) post epost) := by
-  simp only [wp, OrElse.orElse, MonadExcept.orElse]
-  cases x <;> rfl
-
-@[simp] theorem _root_.ExceptT.run_orElse [Monad m] [LawfulMonad m] (x : ExceptT ε m α) (h : Unit → ExceptT ε m α) :
-  (OrElse.orElse x h : ExceptT ε m α).run = (do
-    let r ← x.run
-    match r with
-    | .ok a => pure (.ok a)
-    | .error _ => (h ()).run) := by
-  simp [OrElse.orElse, MonadExcept.orElse]
-
-@[simp]
-theorem orElse_ExceptT_wp [Monad m] [LawfulMonad m] [CompleteLattice l] [WPMonad m l e] (x : ExceptT ε m α) (h : Unit → ExceptT ε m α) :
-  wp x post (epost.1, fun _ => wp (h ()) post epost) ⊑
-    wp (OrElse.orElse x h : ExceptT ε m α) post epost := by
-  apply tryCatch_ExceptT_wp
-
-/-
-@[simp]
-theorem orElse_Option_wp (x : Option α) (h : Unit → Option α) :
-  ∀ post (epost : Prop),
-  wp (OrElse.orElse x h : Option α) post epost =
-    wp x post (wp (h ()) post epost) := by
-  simp only [wp, OrElse.orElse, Option.orElse]
-  cases x <;> simp
--/
-
-@[simp]
-theorem orElse_EStateM_wp (x : EStateM ε σ α) (h : Unit → EStateM ε σ α) :
-  wp (OrElse.orElse x h : EStateM ε σ α) post epost =
-    fun s => wp x post (fun _ s' => wp (h ()) post epost s') s := by
-  funext s
-  simp only [wp, WPMonad.wpImpl, OrElse.orElse, EStateM.orElse]
-  cases x s <;> simp; rfl
-
-/-
-@[simp]
-theorem orElse_OptionT_wp [Monad m] [LawfulMonad m] [CompleteLattice l] [WPMonad m l e] (x : OptionT m α) (h : Unit → OptionT m α) :
-  wp x post (epost.1, wp (h ()) post epost) ⊑
-    wp (OrElse.orElse x h : OptionT m α) post epost := by
-  simp only [wp, OrElse.orElse, OptionT.run]
-  apply PartialOrder.rel_trans; rotate_left; apply WPMonad.wp_bind
-  apply WPMonad.wp_cons (m := m); intro o; cases o with
-  | some a => simp [WPMonad.wp_pure (m := m), PartialOrder.rel_refl]
-  | none => exact PartialOrder.rel_refl
--/
+theorem lift_ExceptT_wp [Monad m] [LawfulMonad m] [CompleteLattice l] [WPMonad m l es]
+    (x : m α) (post : α → l) (epost : EPost ((ε → l) :: es)) :
+  wp (ExceptT.lift x : ExceptT ε m α) post epost = wp (MonadLift.monadLift x : ExceptT ε m α) post epost := rfl
 
 end Loom.WP
